devtools/tests/neg_or.v
@@ -1,26 +1,26 @@
 
+Set Warnings "-native-compiler".
 From Tableaux Require Import All.
 
-Import ATPCompat.
-
 Definition T : EForm :=
-	EOr (EPred "a" []) (ENeg (EPred "a" [])) 
+	EOr (EImp (EPred "a" []) (EOr (EPred "a" []) (ENeg (EPred "a" [])))) (EOr (ENeg (EPred "a" [])) (EPred "a" [])) 
 .
 
 Definition subst := translate_substitution [].
 
 
-Theorem T_proof :
-	hasTableau OuterSkolemization {{  translate_EForm (ENeg T) }} subst.
+Definition T_Proof : ExtendedRuleTree.
 Proof.
-exists \{\}, \{\}.
-eapply hasTableauNegOr with (i := 0).
-1: reflexivity. 
-eapply hasTableauNegNeg with (i := 0).
-1: reflexivity. 
-eapply hasTableauContr with (i := 0) (j := 2).
-1: reflexivity. 
-1: reflexivity. 
-reflexivity.
+apply (mkUnaryNode ( AlphaNegOr (Neg [[ EOr (EImp (EPred "a" []) (EOr (EPred "a" []) (ENeg (EPred "a" [])))) (EOr (ENeg (EPred "a" [])) (EPred "a" [])) ]]) ) ).
+apply (mkUnaryNode ( AlphaNegImp (Neg [[ EImp (EPred "a" []) (EOr (EPred "a" []) (ENeg (EPred "a" []))) ]]) ) ).
+apply (mkUnaryNode ( AlphaNegOr (Neg [[ EOr (ENeg (EPred "a" [])) (EPred "a" []) ]]) ) ).
+exact Leaf.
+Defined.
+
+Theorem hasTableau_T_proof :
+	GuidedTableauSearch InnerSkolemization [  Neg [[ T ]] ]
+subst T_Proof = ret true.
+Proof.
+now native_compute.
 Qed.
 
